\chapter{Polygonal Jordan Curve Theorem: Verified Theorems and Dependencies}
\label{app:JordanVerification}

\section{HOL Light List and Set Library}
Function specifications marked with $\dag$ have been contributed.
\begin{alignat*}{3}
  & \code{head}\,:\,[\alpha] \rightarrow \alpha &\qquad
  & \code{tail}\,:\,[\alpha] \rightarrow [\alpha]\dag &\qquad
  & \code{length}\ [\alpha]\rightarrow \mathbb{N}\\
  & \code{head}\ (\cons{x}{xs}) = x &\qquad
  & \code{tail}\ [] = [] &\qquad
  & \code{length}\ [] = 0\\
  & &\qquad
  &\code{tail}\ (\cons{x}{xs}) = xs &\qquad
  & \code{length}\ (\cons{x}{xs}) = \code{length}\ xs + 1
\end{alignat*}
\begin{align*}
  &\code{butlast}\,:\,[\alpha] \rightarrow [\alpha]\\
  &\code{butlast}\ [] = []\\
  &\code{butlast}\ (\cons{x}{xs}) = \code{if}\ xs=[]\ \code{then}\ []\ \code{else}\ \cons{x}{(\code{butlast}\ xs)}
\end{align*}
\begin{align*}
  &\code{el}\,:\,\code{int} \rightarrow [\alpha] \rightarrow \alpha\\
  &\code{el}\ 0\ xs = \code{head}\ xs\\
  &\code{el}\ (\code{suc}\ n)\ xs = \code{el}\ n\ (\code{tail}\ xs)
\end{align*}
\begin{align*}
  & \code{mem}\,:\,\alpha \rightarrow [\alpha] \rightarrow \code{bool} &\qquad\qquad
  & \code{all}\,:\,(\alpha\rightarrow\code{bool}) \rightarrow [\alpha] \rightarrow \code{bool}\\
  & \code{mem}\ x\ [] = \bot &\qquad\qquad
  & \code{all}\ p\ [] = \bot\\
  & \code{mem}\ x\ (\cons{y}{ys}) = x = y \vee \code{mem}\ x\ ys &\qquad\qquad
  & \code{all}\ p\ (\cons{x}{xs}) = p\ x \wedge \code{all}\ p\ xs   
\end{align*}
\begin{align*}
  & \code{pairwise}\,:\,(\alpha \rightarrow \alpha \rightarrow \code{bool}) \rightarrow [\alpha] \rightarrow \code{bool}\\
  & \code{pairwise}\ R\ [] = \top\\
  & \code{pairwise}\ R\ (\cons{x}{xs}) = \code{all}\ (R x)\ xs \wedge \code{pairwise}\ R\ xs
\end{align*}\\
\begin{align*}
  & \code{zip}\,:\,[\alpha]\rightarrow[\beta]\rightarrow[(\alpha,\beta)] &\quad
  & \code{adjacent}\,:\,[\alpha]\rightarrow[(\alpha,\alpha)]\dag\\
  & \code{zip}\,[]\,[] = [] &\quad
  & \code{adjacent}\,xs = \code{zip}\ (\code{butlast}\ xs)\ (\code{tail}\ xs)\\
  & \code{zip}\,(\cons{x}{xs})(\cons{y}{ys}) = \cons{(x,y)}{\code{zip}\ xs\ ys}
\end{align*}
\begin{align*}
  & \code{disjoint}\,:\,(\alpha\rightarrow\code{bool})\rightarrow(\alpha\rightarrow\code{bool})\rightarrow\code{bool}\\
  & \code{disjoint}\ S\ T = S \cap T = \emptyset
\end{align*}

\section{Polygon Definitions}
\begin{align*}
  &\code{on\_polypath}\,:\,[\code{point}] \rightarrow \code{point} \rightarrow \code{bool}\\
  &\code{on\_polypath}{Ps}{P} \iff\\
  &\quad\code{mem}\ P\ Ps\vee\,\exists x\ y.\; \code{mem}\ (x,y)\ (\code{adjacent}\ Ps) \wedge \between{x}{P}{y}.
\end{align*}

\begin{align*}
  &\code{poly\_path\_connected}\,:\,\code{plane}\rightarrow(\code{point} \rightarrow \code{bool}) \rightarrow \code{point} \rightarrow \code{point} \rightarrow \code{bool}\\
  &\code{poly\_path\_connected}\ \alpha\ figure\ P\ Q \iff\\
  &\quad\exists path.\; path \neq []\\
  &\qquad\wedge\,(\forall R.\ \code{mem}\ R\ path \implies \onplane{R}{\alpha})\\
  &\qquad\wedge\,\code{head}\ path = P \wedge \code{last}\ path = Q\\
  &\qquad\wedge\,\code{disjoint}\ (\code{on\_polypath}\ path)\ figure.
\end{align*}

\begin{align*}
  &\code{simple\_polygon}\,:\,[\code{point}] \rightarrow \code{bool}\\
  &\code{simple\_polygon}\ Ps \iff \\
  &\qquad 3 \leq \code{length}\ Ps\\
  &\qquad\wedge \code{head}\ ps = \code{last}\ Ps\\
  &\qquad\wedge (\forall P.\;\code{mem}\ P\ Ps \implies \code{on\_plane}\ P\ \alpha)\\
  &\qquad\wedge \code{pairwise}\ (\neq)\ (\code{butlast}\ Ps)\\
  &\qquad\wedge \neg(\exists P\;Q\;X.\; \code{mem}\;X\;Ps\wedge\code{mem}\;(P,Q)\;(\code{adjacent}\;Ps)\wedge\between{P}{X}{Q})\\
  &\qquad\wedge \code{pairwise}\ (\lambda(P,Q)\;(P',Q').\;\neg(\exists X. \between{P}{X}{P'} \wedge \between{Q}{X}{Q'}).
\end{align*}

\section{Theorems}
\begin{align*}
\vdash &\code{on\_plane}\ P1\ \alpha \wedge \code{on\_plane}\ P2\ \alpha \wedge \code{on\_plane}\ Q1\ \alpha \wedge \code{on\_plane}\ Q2\ \alpha\\
       &\wedge(\forall X. \code{mem}\ X\ Ps \implies \code{on\_plane}\ X\ \alpha) \wedge (\forall X. \code{mem}\ X\ Qs \implies \code{on\_plane}\ X\ \alpha)\\
       &\wedge\Triangle{a}{P1}{P2}{Q1}\\
       &\wedge\Triangle{a}{Q1}{Q2}{P1}\\
       &\wedge\code{between}\ P1\ X\ P2 \wedge \code{between}\ Q1\ X\ Q2\\
       &\wedge P1 = \code{last}\ (\cons{P2}{Ps}) \wedge Q1 = \code{last}\ (\cons{Q2}{Qs})\\
       &\implies \exists Y. \code{on\_polyseg}\ (\cons{P2}{Ps}\ Y) \wedge \code{on\_polyseg}\ (\cons{Q1}{\cons{Q2}{Qs}})\ Y\\
       &\qquad\vee \code{on\_polyseg}\ (\cons{P1}{\cons{P2}{Ps}})\ Y) \wedge \code{on\_polyseg}\ (\cons{Q2}{Qs})\ Y
\end{align*}

\begin{align*}
\vdash &\code{simple\_polygon}\ \alpha\ Ps\\
       &\implies \exists P\ Q.\; \code{on\_plane}\ P\ \alpha \wedge \code{on\_plane}\ Q\ \alpha\\
       &\qquad\wedge \neg\code{on\_polyseg}\ Ps\ P \wedge \neg\code{on\_polyseg}\ Ps\ Q\\
       &\qquad\wedge \neg\code{seg\_connected}\ \alpha\ (\code{on\_polyseg}\ Ps)\ P\ Q
\end{align*}

\begin{align*}
\vdash &\code{simple\_polygon}\ \alpha\ Ps\\
       &\wedge \code{on\_plane}\ P\ \alpha \wedge \code{on\_plane}\ Q\ \alpha \wedge \code{on\_plane}\ R\ \alpha\\
       &\wedge \neg\code{on\_polyseg}\ Ps\ P\wedge \neg\code{on\_polyseg}\ Ps\ Q\wedge \neg\code{on\_polyseg}\ Ps\ R\\
       &\implies \code{seg\_connected}\ \alpha\ (\code{on\_polyseg}\ Ps)\ P\ Q\\
       &\qquad\quad\vee \code{seg\_connected}\ \alpha\ (\code{on\_polyseg}\ Ps)\ P\ R\\
       &\qquad\quad\vee \code{seg\_connected}\ \alpha\ (\code{on\_polyseg}\ Ps)\ Q\ R
\end{align*}


%    & &\quad
%    & &\quad
%    & &\quad
%    &\quad\code{else}\ \cons{x}{(\code{butlast}\ xs)}
  % \begin{alignedat}{2}
  %   &\code{butlast}\ [] = [] &\qquad & \code{}\ 
  %   &\code{init}

%  &\code{head}\ [] = [] & & & 
%  &\code{head}\ (\cons{x}{xs})
  
%   &\code{tail}\,:\,[\alpha] \rightarrow \alpha\\
%   &\code{tail}\ []             = []\dag\\
%   &\code{tail}\ (\cons{x}{xs}) = xs\\
%   &\code{butlast}\ []             = []\\
%   &\code{butlast}\ (\cons{x}{xs}) = \code{if}\ xs=[]\ \code{then}\ []\\
%                                  &\qquad\code{else}\ \cons{x}{(\code{butlast}\ xs)}\\
%   &\code{length}\ [] = 0\\
%   &\code{length}\ (\cons{x}{xs}) = 1 + \code{length}\ xs\\
%   &\code{last}\ xs = \code{el}\ (\code{length} - 1)\ xs\\
%   &\append{[]}{ys} = ys\\
%   &\append{(\cons{x}{xs})}{ys} = \cons{x}{(\append{xs}{ys})}\\
%   &\code{zip}\ []\  []                = []\\
%   &\code{zip}\ (x:xs)\ (y:ys) = \cons{(x,y)}{\code{zip}\ xs\ ys}\\
%   &\code{all}\ P\ [] \iff \top\\
%   &\code{all}\ P\ (\cons{x}{xs}) \iff P\ h \wedge \code{all}\ xs\\
%   &\code{pairwise}\ P\ [] \iff \top\\
%   &\code{pairwise}\ P\ (\cons{x}{xs}) \iff \code{all}\ (P\ x)\ xs \wedge \code{pairwise}\ xs\\
%   &\code{mem}\ P\ xs \iff \code{set\_of\_list} xs \subseteq P\\
%   &\code{adjacent}\ xs = \code{zip} (\code{butlast}\ xs) (\code{tail}\ xs)\\
%   \\
%   &\code{disjoint}\ s\ t \iff s \cap t = \emptyset
% \end{align*}

% \section{Definition of Polygons}
% \begin{align*}
%   \code{on\_polyseg}\ p\ P \iff \code{mem}\ P\ p \vee \exists x\ y. \code{mem}\ (x,y)\ (\code{adjacent}\ p) \wedge \between{x}{P}{y}
%   \code{head}\ (\cons{x}{xs}) &= x\\
%   \code{tail}\ []             &= []\dag\\
%   \code{tail}\ (\cons{x}{xs}) &= xs\\
%   \code{butlast}\ []             &= []\\
%   \code{butlast}\ (\cons{x}{xs}) &= \code{if}\ xs=[]\ \code{then}\ []\\
%                                  &\qquad\code{else}\ \cons{x}{(\code{butlast}\ xs)}\\
%   \code{length}\ [] &= 0\\
%   \code{length}\ (\cons{x}{xs}) &= 1 + \code{length}\ xs\\
%   \code{last}\ xs &= \code{el}\ (\code{length} - 1)\ xs\\
%   \append{[]}{ys} &= ys\\
%   \append{(\cons{x}{xs})}{ys} &= \cons{x}{(\append{xs}{ys})}\\
%   \code{zip}\ []\  []                &= []\\
%   \code{zip}\ (x:xs)\ (y:ys) &= \cons{(x,y)}{\code{zip}\ xs\ ys}\\
%   \code{all}\ P\ [] &\iff \top\\
%   \code{all}\ P\ (\cons{x}{xs}) &\iff P\ h \wedge \code{all}\ xs\\
%   \code{pairwise}\ P\ [] &\iff \top\\
%   \code{pairwise}\ P\ (\cons{x}{xs}) &\iff \code{all}\ (P\ x)\ xs \wedge \code{pairwise}\ xs\\
%   \code{mem}\ P\ xs &\iff \code{set\_of\_list} xs \subseteq P\\
%   \code{adjacent}\ xs = \code{zip} (\code{butlast}\ xs) (\code{tail}\ xs)\\
%   \\
%   \code{disjoint}\ s\ t \iff& s \cap t = \emptyset
% \end{align*}

%%% Local Variables: 
%%% TeX-master: "../thesis"
%%% End: 
